theories/SetModel/HO_prop.v
@@ -1,0 +1,57 @@
+Require Import library.
+Require Import ZF_axioms ZF_library ZF_nat.
+Require Import HO.
+
+(* Universe of propositions *)
+
+Definition propTy_HO : ZFSet -> ZFSet := fun _ => ⟨ Ω ; ⟨ ZFfour ; ∅ ⟩ ⟩.
+
+Lemma propTy_HO_typing {n : nat} {Γ : ZFSet} : ∀ γ ∈ Γ, propTy_HO γ ∈ 𝕌 n.
+Proof.
+  intros γ Hγ. apply setMkPair_typing.
+  - apply Ω_typing.
+  - apply setMkPair_typing.
+    + apply four_typing.
+    + apply empty_in_univ.
+Qed.
+
+Lemma el_propTy {n : nat} {γ : ZFSet} : 𝕌el n (propTy_HO γ) ≡ Ω.
+Proof.
+  apply setPairβ1.
+  + apply Ω_typing.
+  + apply setMkPair_typing. apply four_typing. apply empty_in_univ.
+Qed.
+
+(* False proposition *)
+
+Definition falseTy_HO : ZFSet -> ZFSet := fun γ => prop FalseS.
+
+Lemma falseTy_HO_typing (Γ : ZFSet) : ∀ γ ∈ Γ, falseTy_HO γ ∈ Ω.
+Proof.
+  intros. cbn. apply prop_typing.
+Qed.
+
+(* Eliminator of False *)
+
+Definition emptyrecTm_HO (A : ZFSet -> ZFSet) (H : ZFSet -> ZFSet) := ∅.
+
+Lemma emptyrecTm_HO_typing {n : nat} {Γ : ZFSet} {A H : ZFSet -> ZFSet}
+  (HA : ∀ γ ∈ Γ, A γ ∈ 𝕌 n) (HH : ∀ γ ∈ Γ, H γ ∈ falseTy_HO γ) :
+  ∀ γ ∈ Γ, emptyrecTm_HO A H ∈ 𝕌el n (A γ).
+Proof.
+  intros γ Hγ. specialize (HH γ Hγ). cbn in HH. apply prop_true_if in HH. destruct HH.
+Qed.
+
+(* Observational equality *)
+
+Definition eqTy_HO (A t u : ZFSet -> ZFSet) : ZFSet -> ZFSet :=
+  fun γ => prop (t γ ≡ u γ).
+
+Definition reflTm_HO (A t : ZFSet -> ZFSet) : ZFSet -> ZFSet := fun _ => ∅.
+
+Lemma eqTy_HO_typing {n : nat} {Γ : ZFSet} {A t u : ZFSet -> ZFSet}
+  (HA : ∀ γ ∈ Γ, A γ ∈ 𝕌 n) (Ht : ∀ γ ∈ Γ, t γ ∈ 𝕌el n (A γ)) (Hu : ∀ γ ∈ Γ, u γ ∈ 𝕌el n (A γ)) :
+  ∀ γ ∈ Γ, eqTy_HO A t u γ ∈ Ω.
+Proof.
+  intros γ Hγ. cbn. apply prop_typing.
+Qed.
