theories/SetModel/HO_univ.v
@@ -1,10 +1,10 @@
 Require Import library.
-Require Import ZF_axioms ZF_library.
+Require Import ZF_axioms ZF_library ZF_nat.
 Require Import HO.
 
 Definition univTy_HO (n : nat) : ZFSet -> ZFSet := fun _ => ⟨ 𝕌 n ; ⟨ ZFthree ; ∅ ⟩ ⟩.
 
-Lemma natTy_HO_typing {n : nat} {Γ : ZFSet} : ∀ γ ∈ Γ, univTy_HO n γ ∈ 𝕌 (S n).
+Lemma univTy_HO_typing {n : nat} {Γ : ZFSet} : ∀ γ ∈ Γ, univTy_HO n γ ∈ 𝕌 (S n).
 Proof.
   intros γ Hγ. apply setMkPair_typing.
   - apply 𝕌_in_𝕍.
