theories/SetModel/ZF_acc.v
@@ -1,0 +1,148 @@
+Require Import library.
+Require Import ZF_axioms ZF_library ZF_nat.
+
+(* Accessibility predicate
+   The code is somewhat technical but not very difficult *)
+
+Definition acc (A : ZFSet) (R : ZFSet -> ZFSet -> SProp) (a : ZFSet) : SProp :=
+  ∀ X ∈ 𝒫 A, (∀ b ∈ A, (∀ c ∈ A, R c b -> c ∈ X) -> b ∈ X) -> a ∈ X.
+
+Lemma acc_intro (A : ZFSet) (R : ZFSet -> ZFSet -> SProp) (a : ZFSet)
+  (Ha : a ∈ A) (IHa : ∀ b ∈ A, R b a -> acc A R b) : acc A R a.
+Proof.
+  intros X HX Hind. apply Hind. assumption.
+  intros b Hb HRb. apply (IHa b Hb HRb X HX Hind).
+Qed.
+
+Lemma acc_ind (A : ZFSet) (R : ZFSet -> ZFSet -> SProp) (P : ZFSet -> SProp)
+  (HP : ∀ a ∈ A, (∀ b ∈ A, R b a -> acc A R b) -> (∀ b ∈ A, R b a -> P b) -> P a)
+  (a : ZFSet) (Ha : a ∈ A) (H : acc A R a) : P a.
+Proof.
+  assert (a ∈ { b ϵ A ∣ acc A R b ∧ P b }).
+  { apply (H { b ϵ A ∣ acc A R b ∧ P b }).
+    - apply ZFinpower. intros b Hb. apply ZFincomp in Hb. now destruct Hb.
+    - intros b Hb IHb. apply ZFincomp. split. 2: split.
+      + assumption.
+      + apply (acc_intro A R b Hb). intros c Hc HRc. specialize (IHb c Hc HRc).
+        apply ZFincomp in IHb. now destruct IHb as [  _ [ H0 _ ] ].
+      + apply (HP b Hb) ; intros c Hc HRc ; specialize (IHb c Hc HRc) ;
+        apply ZFincomp in IHb ; now destruct IHb as [ H0 [ H1 H2 ] ]. }
+  apply ZFincomp in H0. now destruct H0 as [ H0 [ H1 H2 ] ].
+Qed.
+
+Lemma acc_inv (A : ZFSet) (R : ZFSet -> ZFSet -> SProp) {a : ZFSet}
+  (Ha : a ∈ A) (HRa : acc A R a) {b : ZFSet} (Hb : b ∈ A) (HRb : R b a) : acc A R b.
+Proof.
+  revert b Hb HRb. refine (acc_ind A R (fun a => forall b : ZFSet, b ∈ A -> R b a -> acc A R b) _ a Ha HRa).
+  clear a Ha HRa. intros a Ha HRa IHa b Hb HRb. now apply HRa.
+Qed.
+
+Definition accrel (n : nat) (A : ZFSet) (R : ZFSet -> ZFSet -> SProp)
+  (P : ZFSet -> ZFSet) (rec : ZFSet -> ZFSet -> ZFSet) :=
+  { x ϵ setSigma n A P ∣
+      ∀ X ∈ 𝒫 (setSigma n A P),
+      (∀ a ∈ A, ∀ f ∈ { b ϵ A ∣ R b a } ⇒ 𝕍 n, 
+          (∀ b ∈ A, R b a -> acc A R b) -> (∀ b ∈ A, R b a -> ⟨ b ; setAppArr { b ϵ A ∣ R b a } (𝕍 n) f b ⟩ ∈ X) -> ⟨ a ; rec a f ⟩ ∈ X)
+      -> x ∈ X }.
+
+Lemma accrel_intro {n : nat} (A : ZFSet) (R : ZFSet -> ZFSet -> SProp)
+  {P : ZFSet -> ZFSet} {rec : ZFSet -> ZFSet -> ZFSet} (HP : ∀ a ∈ A, P a ∈ 𝕍 n)
+  (Hrec : ∀ a ∈ A, ∀ f ∈ { b ϵ A ∣ R b a } ⇒ 𝕍 n,
+      (∀ b ∈ A, R b a -> acc A R b) -> (∀ b ∈ A, R b a -> setAppArr { b ϵ A ∣ R b a } (𝕍 n) f b ∈ P b) -> rec a f ∈ P a)
+  {a : ZFSet} (Ha : a ∈ A) (HRa : acc A R a) {φ : ZFSet} (Hφ : φ ∈ { b ϵ A ∣ R b a } ⇒ 𝕍 n)
+  (Hφ2 : ∀ b ∈ A, R b a -> ⟨ b ; setAppArr { b ϵ A ∣ R b a } (𝕍 n) φ b ⟩ ∈ accrel n A R P rec) :
+  ⟨ a ; rec a φ ⟩ ∈ accrel n A R P rec.
+Proof.
+  apply ZFincomp. split.
+  - apply setMkSigma_typing ; try assumption. apply Hrec ; try assumption.
+    + now apply acc_inv.
+    + intros b Hb HRb. specialize (Hφ2 b Hb HRb). apply ZFincomp in Hφ2. destruct Hφ2 as [ Hφ2 _ ].
+      apply setMkSigma_detyping in Hφ2. now destruct Hφ2. exact HP.
+  - intros X HX Hind. apply Hind ; try assumption.
+    + now apply acc_inv.
+    + intros b Hb HRb. specialize (Hφ2 b Hb HRb). apply ZFincomp in Hφ2. destruct Hφ2 as [ _ Hφ2 ].
+      apply (Hφ2 X HX Hind).
+Qed.
+
+Definition accrelU (n : nat) (A : ZFSet) (R : ZFSet -> ZFSet -> SProp)
+  (P : ZFSet -> ZFSet) (rec : ZFSet -> ZFSet -> ZFSet) (a : ZFSet) (φ : ZFSet) :=
+  { x ϵ accrel n A R P rec ∣ setFstSigma n A P x ≡ a -> setSndSigma n A P x ≡ rec a φ }.
+
+Lemma accrelU_intro {n : nat} (A : ZFSet) (R : ZFSet -> ZFSet -> SProp)
+  {P : ZFSet -> ZFSet} {rec : ZFSet -> ZFSet -> ZFSet} {a α : ZFSet} {φ ψ : ZFSet} (HP : ∀ a ∈ A, P a ∈ 𝕍 n)
+  (Hrec : ∀ a ∈ A, ∀ f ∈ { b ϵ A ∣ R b a } ⇒ 𝕍 n,
+      (∀ b ∈ A, R b a -> acc A R b) -> (∀ b ∈ A, R b a -> setAppArr { b ϵ A ∣ R b a } (𝕍 n) f b ∈ P b) -> rec a f ∈ P a)
+  (Ha : a ∈ A) (HRa : acc A R a)
+  (Hφ : φ ∈ { b ϵ A ∣ R b a } ⇒ 𝕍 n) (Hφ2 : ∀ b ∈ A, R b a -> ⟨ b ; setAppArr { b ϵ A ∣ R b a } (𝕍 n) φ b ⟩ ∈ accrelU n A R P rec α ψ)
+  (Hψ : ψ ∈ { b ϵ A ∣ R b α } ⇒ 𝕍 n) (Hψ2 : ∀ b ∈ A, R b α -> ⟨ b ; setAppArr { b ϵ A ∣ R b α } (𝕍 n) ψ b ⟩ ∈ accrel n A R P rec)
+  (Hψu : ∀ b ∈ A, R b α -> ∀ pb ∈ P b, ⟨ b ; pb ⟩ ∈ accrel n A R P rec -> pb ≡ setAppArr { b ϵ A ∣ R b α } (𝕍 n) ψ b) :
+  ⟨ a ; rec a φ ⟩ ∈ accrelU n A R P rec α ψ.
+Proof.
+  apply ZFincomp. split.
+  - apply accrel_intro ; try assumption. intros b Hb HRb. specialize (Hφ2 b Hb HRb).
+    apply ZFincomp in Hφ2. now destruct Hφ2.
+  - intro H. assert (∀ b ∈ A, R b a -> setAppArr {b ϵ A ∣ R b a} (𝕍 n) φ b ∈ P b) as Hφ3.
+    { intros b Hb HRb. specialize (Hφ2 b Hb HRb). apply ZFincomp in Hφ2. destruct Hφ2 as [ Hφ2 _ ].
+      apply ZFincomp in Hφ2. destruct Hφ2 as [ Hφ2 _ ]. apply setMkSigma_detyping in Hφ2.
+      now destruct Hφ2. assumption. }
+    assert (setFstSigma n A P ⟨ a; rec a φ ⟩ ≡ a) as H0.
+    { apply setSigmaβ1 ; try assumption. apply Hrec ; try assumption. now apply acc_inv. }
+    pose proof (trans (sym H) H0) as H1. clear H H0. destruct H1.
+    assert (setSndSigma n A P ⟨ α ; rec α φ ⟩ ≡ rec α φ) as H0.
+    { apply setSigmaβ2 ; try assumption. apply Hrec ; try assumption. now apply acc_inv. }
+    refine (trans H0 _). clear H0. assert (φ ≡ ψ) as Hφψ.
+    { apply (setArr_funext Hφ Hψ). intros b Hb. apply ZFincomp in Hb. destruct Hb as [ Hb HRb ].
+      refine (Hψu b Hb HRb (setAppArr {b0 ϵ A ∣ R b0 α} (𝕍 n) φ b) _ _).
+      1,2: specialize (Hφ2 b Hb HRb) ; apply ZFincomp in Hφ2 ; destruct Hφ2 as [ Hφ2 _ ].
+      now apply Hφ3. assumption. }
+    destruct Hφψ. reflexivity.
+Qed.
+
+Lemma accrel_incl_accrelU {n : nat} (A : ZFSet) (R : ZFSet -> ZFSet -> SProp)
+  {P : ZFSet -> ZFSet} {rec : ZFSet -> ZFSet -> ZFSet} {α : ZFSet} {ψ : ZFSet} (HP : ∀ a ∈ A, P a ∈ 𝕍 n)
+  (Hrec : ∀ a ∈ A, ∀ f ∈ { b ϵ A ∣ R b a } ⇒ 𝕍 n,
+      (∀ b ∈ A, R b a -> acc A R b) -> (∀ b ∈ A, R b a -> setAppArr { b ϵ A ∣ R b a } (𝕍 n) f b ∈ P b) -> rec a f ∈ P a)
+  (Hψ : ψ ∈ { b ϵ A ∣ R b α } ⇒ 𝕍 n) (Hψ2 : ∀ b ∈ A, R b α -> ⟨ b ; setAppArr { b ϵ A ∣ R b α } (𝕍 n) ψ b ⟩ ∈ accrel n A R P rec)
+  (Hψu : ∀ b ∈ A, R b α -> ∀ pb ∈ P b, ⟨ b ; pb ⟩ ∈ accrel n A R P rec -> pb ≡ setAppArr { b ϵ A ∣ R b α } (𝕍 n) ψ b) :
+  accrel n A R P rec ⊂ accrelU n A R P rec α ψ.
+Proof.
+  intros x Hx. pose proof Hx as Hx2. apply ZFincomp in Hx2. destruct Hx2 as [ Hx2 Hx3 ]. apply Hx3.
+  - clear x Hx Hx2 Hx3. apply ZFinpower. intros x Hx. apply ZFincomp in Hx.
+    destruct Hx as [ Hx _ ]. apply ZFincomp in Hx. now destruct Hx as [ Hx _ ].
+  - intros a Ha φ Hφ HRa IHa. apply accrelU_intro ; try assumption.
+    now apply acc_intro. 
+Qed.
+
+Lemma accrel_funrel {n : nat} (A : ZFSet) (R : ZFSet -> ZFSet -> SProp)
+  {P : ZFSet -> ZFSet} {rec : ZFSet -> ZFSet -> ZFSet} (HP : ∀ a ∈ A, P a ∈ 𝕍 n)
+  (Hrec : ∀ a ∈ A, ∀ f ∈ { b ϵ A ∣ R b a } ⇒ 𝕍 n,
+      (∀ b ∈ A, R b a -> acc A R b) -> (∀ b ∈ A, R b a -> setAppArr { b ϵ A ∣ R b a } (𝕍 n) f b ∈ P b) -> rec a f ∈ P a)
+  {a : ZFSet} (Ha : a ∈ A) (HRa : acc A R a) : ∃! pa ∈ P a, ⟨ a ; pa ⟩ ∈ accrel n A R P rec.
+Proof.
+  unshelve eapply (acc_ind A R (fun a => ∃! pa ∈ P a, ⟨ a ; pa ⟩ ∈ accrel n A R P rec) _ a Ha HRa).
+  clear a Ha HRa. intros a Ha HRa IHa.
+  set (Rφ := fun x px => px ∈ P x ∧ ⟨ x ; px ⟩ ∈ accrel n A R P rec).
+  assert (isFunRel { b ϵ A ∣ R b a } (𝕍 n) Rφ) as HRφ.
+  { intros b Hb. apply ZFincomp in Hb. destruct Hb as [ Hb HRb ]. specialize (IHa b Hb HRb).
+    destruct IHa as [ pb [ [ Hpb Hpb2 ] Hpb3 ] ]. exists pb. split.
+    - split. eapply ZFuniv_trans. exact Hpb. now apply HP. now split.
+    - intros pb' [ Hpb' [ Hpb'2 Hpb'3 ] ]. now apply Hpb3. }
+  set (φ := relToGraph { b ϵ A ∣ R b a } (𝕍 n) Rφ).
+  assert (φ ∈ { b ϵ A ∣ R b a } ⇒ (𝕍 n)) as Hφ.
+  { now apply relToGraph_typing. }
+  assert (∀ b ∈ A, R b a -> ⟨ b ; setAppArr { b ϵ A ∣ R b a } (𝕍 n) φ b ⟩ ∈ accrel n A R P rec) as Hφ2.
+  { intros b Hb HRb. unshelve epose proof (funRelApp_inRel (a := b) HRφ _).
+    - apply ZFincomp. now split.
+    - destruct H as [ _ H ]. refine (transpS (fun X => ⟨ b ; X ⟩ ∈ _) (sym _) H). admit. }
+  assert (∀ b ∈ A, R b a -> ∀ pb ∈ P b, ⟨ b ; pb ⟩ ∈ accrel n A R P rec -> pb ≡ setAppArr { b ϵ A ∣ R b a } (𝕍 n) φ b) as Hφu.
+  { intros b Hb HRb pb Hpb Hpb2. unfold isFunRel in HRφ. admit. }
+  assert (⟨ a; rec a φ ⟩ ∈ accrel n A R P rec) as H.
+  { apply accrel_intro ; try assumption. now apply acc_intro. }
+  exists (rec a φ). split.
+  - split ; try assumption. apply Hrec ; try assumption. admit.
+  - intros pa [ Hpa H0 ]. apply (accrel_incl_accrelU A R HP Hrec Hφ Hφ2 Hφu) in H0.
+    apply ZFincomp in H0. destruct H0 as [ H0 H1 ]. unshelve refine (trans (sym (H1 _)) _).
+    + now apply setSigmaβ1.
+    + now apply setSigmaβ2. 
+Qed.
+
